ass 3

test.dfy
@@ -1,7 +1,22 @@
-/* A set is represented as a sequence with no duplicates */
-predicate isSet(s: seq<int>) {
-  forall i: int :: 0 <= i < |s| ==>
-  forall j: int :: 0 <= j < |s| && j != i ==> 
-  s[j] != s[i]
-}
+// /* A set is represented as a sequence with no duplicates */
+// predicate isSet(s: seq<int>) {
+//   forall i: int :: 0 <= i < |s| ==>
+//   forall j: int :: 0 <= j < |s| && j != i ==> 
+//   s[j] != s[i]
+// }
 
+
+// method test(s: seq<int>) returns (t: seq<int>)
+//   ensures s == t
+// {
+//   t := [];
+//   var i := 0;
+//   while i < |s|
+//     invariant 0 <= i <= |s|
+//     invariant t == s[..i]
+//     invariant |t| == i
+//   {
+//     t := t + [s[i]];
+//     i := i + 1;
+//   }
+// }
